---
title: "EJERCICIOS C3T5"
author:
- Betancourt Alison
- Angulo Javier
- Anrango Stalin
- Huilca Fernando
- Sarasti Sebastian
- Simbaña Mateo
toc: true
toc-title: "Contenido"
number-sections: true   
highlight-style: pygments
format:
  html:
    code-fold: true
    embed-resources: true
    html-math-method: katex
  pdf:
    code-line-numbers: true
    geometry: 
      - top=30mm
      - left=30mm
  docx: default
---

## Ejercicio 30

Pruebe la ecuación (6.7.5) por inducción
$$
\begin{align*}
\ \sum_{K=1}^{n+1} K C\cdot \binom{n+1}{K} &= \sum_{k=1}^{n} \left( K \cdot \binom{n}{k-1} + \binom{n}{k} \right) + (n+1) \cdot \binom{n+1}{n+1}
\end{align*}
$$
$$
\begin{align*}
 &= \sum_{k=1}^{n+1} \binom{n}{k-1} + \sum_{k=1}^{n+1} \binom{n}{k}
\end{align*}
$$
$$
\begin{align*}
 &= \sum_{k=1}^{n+1} (k-1) \cdot \binom{n}{k-1} + \sum_{k=1}^{n+1} \binom{n}{k-1} + \sum_{k=1}^{n} \binom{n}{k}
\end{align*}
$$
$$
\begin{align*}
&=   n2^{n-1} + 2^n + n^2 \cdot 2^{n-1} = (n+1) \cdot 2^n
\end{align*}
$$
